ulib/FStar.ST.fst
@@ -30,9 +30,11 @@ let gst_wp (a:Type)   = st_wp_h heap a
 unfold let lift_div_gst (a:Type0) (wp:pure_wp a) (p:gst_post a) (h:heap) = wp (fun a -> p a h)
 sub_effect DIV ~> GST = lift_div_gst
 
-let heap_rel (h1:heap) (h2:heap) =
+let heap_rel0 (h1:heap) (h2:heap) =
   forall (a:Type0) (rel:preorder a) (r:mref a rel). h1 `contains` r ==>
                                                (h2 `contains` r /\ rel (sel h1 r) (sel h2 r))
+
+let heap_rel : preorder heap = heap_rel0
 
 assume val gst_get: unit    -> GST heap (fun p h0 -> p h0 h0)
 assume val gst_put: h1:heap -> GST unit (fun p h0 -> heap_rel h0 h1 /\ p () h1)
